cakeml-semantics/cakeml_semanticsProofScript.sml
@@ -1,0 +1,386 @@
+(* Relating the itree- and FFI state-based CakeML semantics *)
+open HolKernel Parse boolLib bossLib BasicProvers dep_rewrite;
+open optionTheory relationTheory pairTheory listTheory;
+open lem_pervasives_extraTheory libTheory namespaceTheory astTheory
+     ffiTheory semanticPrimitivesTheory smallStepTheory;
+open io_treeTheory cakeml_semanticsTheory;
+
+val _ = new_theory "cakeml_semanticsProof";
+
+(* TODO use evaluatePropsTheory and semanticPrimitivesPropsTheory *)
+
+(* Deliberately no `application_def` here *)
+val smallstep_ss = simpLib.named_rewrites "smallstep_ss" [
+    smallStepTheory.continue_def,
+    smallStepTheory.return_def,
+    smallStepTheory.push_def,
+    smallStepTheory.e_step_def
+    ];
+
+val itree_ss = simpLib.named_rewrites "itree_ss" [
+    cakeml_semanticsTheory.continue_def,
+    cakeml_semanticsTheory.return_def,
+    cakeml_semanticsTheory.push_def,
+    cakeml_semanticsTheory.estep_def
+    ];
+
+(* Adapt CakeML's RTC definitions to our more functional definitions *)
+Definition step_n_cml_def:
+  step_n_cml 0 e = e ∧
+  step_n_cml (SUC n) (Estep st) = step_n_cml n (e_step st) ∧
+  step_n_cml _ e = e
+End
+
+Theorem step_n_cml_alt_def:
+  step_n_cml 0 e = e ∧
+  step_n_cml (SUC n) e = (
+    case step_n_cml n e of
+    | Estep st => e_step st
+    | e => e)
+Proof
+  rw[step_n_cml_def] >>
+  qid_spec_tac `e` >> qid_spec_tac `n` >>
+  Induct >> Cases >> rewrite_tac[step_n_cml_def] >> simp[]
+QED
+
+Theorem e_step_reln_eq_step_n_cml:
+  e_step_reln^* st1 st2 ⇔
+  ∃n. step_n_cml n (Estep st1) = Estep st2
+Proof
+  reverse $ eq_tac >> rw[] >> pop_assum mp_tac
+  >- (
+    map_every qid_spec_tac [`st2`,`st1`,`n`] >>
+    Induct >> rw[step_n_cml_alt_def] >>
+    EVERY_CASE_TAC >> gvs[] >>
+    rw[Once relationTheory.RTC_CASES2] >> disj2_tac >>
+    last_x_assum $ irule_at Any >> gvs[e_step_reln_def]
+    )
+  >- (
+    Induct_on `RTC e_step_reln` >> rw[]
+    >- (qexists_tac `0` >> gvs[step_n_cml_def])
+    >- (qexists_tac `SUC n` >> gvs[step_n_cml_def, e_step_reln_def])
+    )
+QED
+
+Definition is_halt_cml_def:
+  is_halt_cml (Estep (env, st_ffi, Val v, [])) = T ∧
+  is_halt_cml (Estep (env, st_ffi, Val v, [Craise (), env'])) = T ∧
+  is_halt_cml (Eabort a) = T ∧
+  is_halt_cml _ = F
+End
+
+Definition step_to_halt_cml_def:
+  step_to_halt_cml env st_ffi ev cs =
+    case some n. is_halt_cml (step_n_cml n (Estep (env, st_ffi, ev, cs))) of
+    | NONE => NONE
+    | SOME n => SOME $ step_n_cml n (Estep (env, st_ffi, ev, cs))
+End
+
+Theorem small_eval_eq_step_to_halt_cml:
+  (small_eval env st_ffi e cs (st_ffi', Rval v) ⇔
+  ∃n env'.
+    step_n_cml n (Estep (env, st_ffi, Exp e, cs)) =
+      (Estep (env', st_ffi', Val v, []))) ∧
+  (small_eval env st_ffi e cs (st_ffi', Rerr (Rraise v)) ⇔
+  ∃n env' env''.
+    step_n_cml n (Estep (env, st_ffi, Exp e, cs)) =
+      (Estep (env', st_ffi', Val v, [(Craise (), env'')]))) ∧
+  ((∃st_ffi'. small_eval env st_ffi e cs (st_ffi', Rerr (Rabort a))) ⇔
+  ∃n env' env''.
+    step_n_cml n (Estep (env, st_ffi, Exp e, cs)) = Eabort a)
+Proof
+  reverse $ rw[small_eval_def, e_step_reln_eq_step_n_cml]
+  >- (
+    eq_tac >> rw[]
+    >- (qexists_tac `SUC n` >> gvs[step_n_cml_alt_def]) >>
+    Induct_on `n` >> gvs[step_n_cml_alt_def] >>
+    EVERY_CASE_TAC >> gvs[] >> rw[PULL_EXISTS] >>
+    PairCases_on `p` >> goal_assum drule >> simp[]
+    ) >>
+  eq_tac >> rw[] >> ntac 2 $ goal_assum drule
+QED
+
+Triviality Estep_is_halt_imp_e_step_neq_Estep:
+  is_halt_cml (Estep st) ⇒ ∀st'. e_step st ≠ Estep st'
+Proof
+  PairCases_on `st` >> rw[] >>
+  Cases_on `st3` >> Cases_on `st4` >> gvs[is_halt_cml_def]
+  >- simp[e_step_def, SF smallstep_ss] >>
+  PairCases_on `h` >>
+  Cases_on `h0` >> Cases_on `t` >> gvs[is_halt_cml_def] >>
+  simp[e_step_def, SF smallstep_ss]
+QED
+
+Theorem application_not_Estuck:
+  application op env st_ffi vs cs ≠ Estuck
+Proof
+  rw[smallStepTheory.application_def] >> EVERY_CASE_TAC >> gvs[SF smallstep_ss]
+QED
+
+Theorem e_step_to_Estuck:
+  e_step (env, st_ffi, ev, cs) = Estuck ⇔
+  (∃v. ev = Val v ∧ cs = []) ∨
+  (∃v env'. ev = Val v ∧ cs = [Craise (), env'])
+Proof
+  reverse $ eq_tac
+  >- (rw[] >> gvs[SF smallstep_ss]) >>
+  gvs[e_step_def] >> CASE_TAC >> gvs[]
+  >- (EVERY_CASE_TAC >> gvs[SF smallstep_ss, application_not_Estuck]) >>
+  Cases_on `cs` >> gvs[SF smallstep_ss] >>
+  EVERY_CASE_TAC >> gvs[application_not_Estuck]
+QED
+
+Theorem e_diverges_eq_step_to_halt_cml:
+  e_diverges env st_ffi e ⇔ step_to_halt_cml env st_ffi (Exp e) [] = NONE
+Proof
+  rw[step_to_halt_cml_def, e_diverges_def, e_step_reln_eq_step_n_cml] >>
+  simp[PULL_EXISTS] >>
+  eq_tac >> rw[] >> gvs[e_step_reln_def]
+  >- (
+    DEEP_INTRO_TAC some_intro >> rw[] >>
+    Induct_on `x` >> rw[] >> gvs[step_n_cml_alt_def, is_halt_cml_def] >>
+    CASE_TAC >> gvs[is_halt_def] >>
+    PairCases_on `p` >> rename1 `Estep (a, b, c, d)` >>
+    last_assum drule >> strip_tac >> gvs[] >> rename1 `Estep (f, g, h, i)` >>
+    last_x_assum $ qspecl_then [`f`,`g`,`h`,`i`,`SUC x`] assume_tac >>
+    gvs[step_n_cml_alt_def] >>
+    metis_tac[Estep_is_halt_imp_e_step_neq_Estep]
+    )
+  >- (
+    last_x_assum mp_tac >>
+    DEEP_INTRO_TAC some_intro >> rw[] >>
+    first_assum $ qspec_then `n` assume_tac >>
+    first_x_assum $ qspec_then `SUC n` assume_tac >> gvs[step_n_cml_alt_def] >>
+    Cases_on `e_step (env', s', e', c')` >> gvs[is_halt_cml_def]
+    >- (PairCases_on `p` >> simp[]) >>
+    gvs[e_step_to_Estuck, is_halt_cml_def]
+    )
+QED
+
+
+(****************************************)
+
+
+Inductive result_rel:
+  result_rel (Rval v) (Rval v) ∧
+  result_rel (Rraise v) (Rerr $ Rraise v)
+End
+
+(* Takes 30s *)
+Theorem do_app_rel:
+  (∀s. op ≠ FFI s) ⇒
+  OPTREL (λ(a,b) (c,d). a = c ∧ result_rel b d)
+    (do_app st op vs)
+    (OPTION_MAP (λ(a,b). (FST a, b)) (do_app (st, ffi) op vs))
+Proof
+  rw[semanticPrimitivesTheory.do_app_def] >>
+  rpt (
+    TOP_CASE_TAC >>
+    gvs[do_app_def, result_rel_cases, store_alloc_def]
+    )
+QED
+
+Inductive ctxt_frame_rel:
+  ctxt_frame_rel Craise (Craise ()) ∧
+  ctxt_frame_rel (Chandle pes) (Chandle () pes) ∧
+  ctxt_frame_rel (Capp op vs es) (Capp op vs () es) ∧
+  ctxt_frame_rel (Clog lop e) (Clog lop () e) ∧
+  ctxt_frame_rel (Cif e1 e2) (Cif () e1 e2) ∧
+  ctxt_frame_rel (Cmat_check pes v) (Cmat_check () pes v) ∧
+  ctxt_frame_rel (Cmat pes v) (Cmat () pes v) ∧
+  ctxt_frame_rel (Clet vopt e) (Clet vopt () e) ∧
+  ctxt_frame_rel (Ccon idopt vs es) (Ccon idopt vs () es) ∧
+  ctxt_frame_rel (Ctannot ty) (Ctannot () ty) ∧
+  ctxt_frame_rel (Clannot ls) (Clannot () ls)
+End
+
+Definition ctxt_rel_def:
+  ctxt_rel cs1 cs2 =
+    LIST_REL (λ(c1,env1) (c2,env2). ctxt_frame_rel c1 c2 ∧ env1 = env2) cs1 cs2
+End
+
+Inductive step_result_rel:
+  (ctxt_rel cs1 cs2 ⇒
+    step_result_rel (Estep (env, st, ev, cs1)) (Estep (env, (st, ffi), ev, cs2))) ∧
+  step_result_rel Edone Estuck ∧
+  step_result_rel Etype_error (Eabort $ Rtype_error)
+End
+
+(* Takes 20s *)
+Theorem application_rel:
+  (∀s. op ≠ FFI s) ∧
+  ctxt_rel cs1 cs2 ⇒
+  step_result_rel
+    (application op env st vs cs1)
+    (application op env (st,ffi) vs cs2)
+Proof
+  rw[] >>
+  drule do_app_rel >> disch_then $ qspecl_then [`vs`,`st`,`ffi`] assume_tac >>
+  rw[application_def, smallStepTheory.application_def] >>
+  rpt (
+    TOP_CASE_TAC >>
+    gvs[step_result_rel_cases, result_rel_cases, ctxt_rel_def,
+        ctxt_frame_rel_cases, SF smallstep_ss, SF itree_ss]
+    ) >>
+  metis_tac[PAIR]
+QED
+
+Triviality application_FFI_results:
+  application (FFI s) env st vs cs = res ⇒
+  res = Etype_error ∨ ∃conf ws lnum. res = Effi s conf ws lnum env st cs
+Proof
+  rw[application_def] >> EVERY_CASE_TAC >> gvs[]
+QED
+
+Theorem application_rel_FFI_type_error:
+  application (FFI s) env st vs cs1 = Etype_error ⇔
+  application (FFI s) env (st, ffi) vs cs2 = Eabort Rtype_error
+Proof
+  rw[application_def, smallStepTheory.application_def] >>
+  simp[semanticPrimitivesTheory.do_app_def] >>
+  EVERY_CASE_TAC >> gvs[SF smallstep_ss] >>
+  gvs[store_lookup_def, store_assign_def, store_v_same_type_def]
+QED
+
+Theorem application_rel_FFI:
+  application (FFI s) env st vs cs1 = Effi s conf ws lnum env st cs1 ⇒
+  ∃ws.
+    store_lookup lnum st = SOME $ W8array ws ∧
+    application (FFI s) env (st, ffi) vs cs2 =
+      if s = "" then Estep (env, (st, ffi), Val $ Conv NONE [], cs2) else
+      case ffi.oracle s ffi.ffi_state conf ws of
+      | Oracle_return ffi' ws' =>
+          if LENGTH ws' ≠ LENGTH ws then
+            Eabort $ Rffi_error $ Final_event s conf ws FFI_failed
+          else
+            Estep (env,
+              (LUPDATE (W8array ws') lnum st,
+               ffi with <|
+                  ffi_state := ffi';
+                  io_events := ffi.io_events ++ [IO_event s conf (ZIP (ws,ws'))]
+                  |>),
+              Val $ Conv NONE [], cs2)
+      | Oracle_final outcome =>
+          Eabort $ Rffi_error $ Final_event s conf ws outcome
+Proof
+  simp[application_def] >>
+  ntac 6 (TOP_CASE_TAC >> gvs[]) >>
+  gvs[store_lookup_def] >>
+  ntac 2 (TOP_CASE_TAC >> gvs[]) >> rw[] >>
+  goal_assum drule >>
+  simp[smallStepTheory.application_def, semanticPrimitivesTheory.do_app_def] >>
+  simp[store_lookup_def, call_FFI_def] >>
+  reverse IF_CASES_TAC >> gvs[store_assign_def, store_v_same_type_def]
+  >- (simp[SF smallstep_ss] >> drule LUPDATE_SAME >> gvs[]) >>
+  qmatch_goalsub_abbrev_tac `foo l` >>
+  reverse $ Cases_on `foo l` >> gvs[] >>
+  IF_CASES_TAC >> gvs[SF smallstep_ss]
+QED
+
+Theorem application_rel_FFI':
+  application (FFI s) env (st, ffi) vs cs2 ≠ Eabort Rtype_error ⇒
+  ∃conf lnum ws.
+    vs = [Litv $ StrLit conf; Loc lnum] ∧
+    store_lookup lnum st = SOME $ W8array ws ∧
+    application (FFI s) env st vs cs1 =
+      Effi s (MAP (λc. n2w $ ORD c) (EXPLODE conf)) ws lnum env st cs1
+Proof
+  rw[smallStepTheory.application_def, semanticPrimitivesTheory.do_app_def] >>
+  EVERY_CASE_TAC >> gvs[application_def]
+QED
+
+Theorem do_app_ffi_changed:
+  do_app (st, ffi) op vs = SOME ((st', ffi'), res) ∧
+  ffi ≠ ffi' ⇒
+  ∃s conf lnum ws ffi_st ws'.
+    op = FFI s ∧
+    vs = [Litv (StrLit conf); Loc lnum] ∧
+    store_lookup lnum st = SOME (W8array ws) ∧
+    s ≠ "" ∧
+    ffi.oracle s ffi.ffi_state (MAP (λc. n2w $ ORD c) (EXPLODE conf)) ws =
+      Oracle_return ffi_st ws' ∧
+    LENGTH ws = LENGTH ws'
+Proof
+  simp[semanticPrimitivesTheory.do_app_def] >>
+  EVERY_CASE_TAC >> gvs[store_alloc_def, store_assign_def] >>
+  strip_tac >> gvs[call_FFI_def] >>
+  EVERY_CASE_TAC >> gvs[]
+QED
+
+Theorem do_app_ffi_unchanged:
+  ∀st ffi op vs st' ffi' res.
+    (∀s. op ≠ FFI s) ∧
+    do_app (st, ffi) op vs = SOME ((st', ffi'), res)
+  ⇒ ffi = ffi'
+Proof
+  rpt gen_tac >>
+  simp[semanticPrimitivesTheory.do_app_def] >>
+  EVERY_CASE_TAC >> gvs[store_alloc_def]
+QED
+
+Theorem application_ffi_unchanged:
+  ∀op env st ffi vs cs env' st' ffi' ev cs'.
+    (∀s. op ≠ FFI s) ∧
+    application op env (st, ffi) vs cs = Estep (env', (st', ffi'), ev, cs')
+  ⇒ ffi = ffi'
+Proof
+  rpt gen_tac >>
+  rw[smallStepTheory.application_def, SF smallstep_ss] >>
+  qspecl_then [`st`,`ffi`,`op`,`vs`] assume_tac do_app_ffi_unchanged >>
+  EVERY_CASE_TAC >> gvs[]
+QED
+
+Theorem e_step_ffi_changed:
+  e_step (env, (st, ffi), ev, cs) = Estep (env', (st', ffi'), ev', cs') ∧
+  ffi ≠ ffi' ⇒
+  ∃ s conf lnum env'' ccs ws ffi_st ws'.
+    ev = Val (Litv (StrLit conf)) ∧
+    cs = (Capp (FFI s) [Loc lnum] () [], env'') :: ccs ∧
+    store_lookup lnum st = SOME (W8array ws) ∧
+    s ≠ "" ∧
+    ffi.oracle s ffi.ffi_state (MAP (λc. n2w $ ORD c) (EXPLODE conf)) ws =
+      Oracle_return ffi_st ws' ∧
+    LENGTH ws = LENGTH ws'
+Proof
+  simp[e_step_def] >>
+  EVERY_CASE_TAC >> gvs[SF smallstep_ss]
+  >- (
+    strip_tac >> rename1 `application op _ _ _ _` >>
+    Cases_on `∀s. op ≠ FFI s` >> gvs[]
+    >- (irule application_ffi_unchanged >> rpt $ goal_assum drule) >>
+    gvs[smallStepTheory.application_def, semanticPrimitivesTheory.do_app_def]
+    ) >>
+  EVERY_CASE_TAC >> gvs[] >>
+  rename1 `application op _ _ _ _` >>
+  (
+    strip_tac >> Cases_on `∀s. op ≠ FFI s` >> gvs[]
+    >- (drule_all application_ffi_unchanged >> gvs[]) >>
+    gvs[smallStepTheory.application_def,
+        semanticPrimitivesTheory.do_app_def, call_FFI_def] >>
+    EVERY_CASE_TAC >> gvs[SF smallstep_ss]
+  )
+QED
+
+
+(****************************************)
+
+
+(* Play out a particular trace prefix from a given itree, modelling the
+   environment as an FFI oracle with associated FFI state (as in CakeML) *)
+Definition trace_prefix_def:
+  trace_prefix 0 (oracle, st) itree = ([], NONE) ∧
+  trace_prefix (SUC n) (oracle, st) (Ret r) = ([], SOME r) ∧
+  trace_prefix (SUC n) (oracle, st) (Vis (s, conf, ws) f) =
+    case oracle s st conf ws of
+    | Oracle_return st' ws' =>
+        let (io, res) = trace_prefix n (oracle, st) (f $ INR ws') in
+        (IO_event s conf (ZIP (ws,ws'))::io, res)
+    | Oracle_final outcome => trace_prefix n (oracle, st) (f $ INL outcome)
+End
+
+
+(****************************************)
+
+
+val _ = export_theory();
+
